coq-verification/src/Concrete/Api/Proofs.v
@@ -24,15 +24,6 @@ Require Import Hafnium.Concrete.Assumptions.Mpool.
 Require Import Hafnium.Concrete.Api.Implementation.
 Require Import Hafnium.Concrete.MM.Proofs.
 
-Lemma api_clear_memory_valid
-      {cp : concrete_params} (conc : concrete_state) begin end_ ppool :
-  is_valid conc ->
-  let conc' := snd (fst (api_clear_memory conc begin end_ ppool)) in
-  is_valid conc'.
-Proof.
-  tauto. (* N.B. this proof is trivial because is_valid isn't yet filled in *)
-Qed.
-
 Lemma api_clear_memory_represents
       {ap : @abstract_state_parameters paddr_t nat} {cp : concrete_params}
       {cp_ok : params_valid}
@@ -54,16 +45,6 @@ Proof.
          | _ => apply mm_identity_map_represents
          | _ => solver
          end.
-Qed.
-
-Lemma api_share_memory_valid
-      {cp : concrete_params} (conc : concrete_state)
-      vid addr size share current :
-  is_valid conc ->
-  let conc' := snd (api_share_memory conc vid addr size share current) in
-  is_valid conc'.
-Proof.
-  tauto. (* N.B. this proof is trivial because is_valid isn't yet filled in *)
 Qed.
 
 Lemma api_share_memory_represents
